PR comment fixes

AML_definition.v
@@ -1,5 +1,7 @@
 Require Import String.
 Require Import Coq.Lists.ListSet.
+Require Import Coq.Sets.Ensembles.
+Require Import Ensembles_Ext.
 
 Section AML.
 
@@ -8,26 +10,29 @@ Inductive SVar : Type := svar_c {id_sv : string}.
 Inductive Sigma : Type := sigma_c {id_si : string}.
 
 Inductive Sigma_pattern : Type :=
-  | sp_var (x : EVar)
-  | sp_set (X : SVar)
-  | sp_const (sigma : Sigma)
-  | sp_app (phi1 phi2 : Sigma_pattern)
-  | sp_bottom
-  | sp_impl (phi1 phi2 : Sigma_pattern)
-  | sp_exists (x : EVar) (phi : Sigma_pattern)
-  | sp_mu (X : SVar) (phi : Sigma_pattern)
+| sp_var (x : EVar)
+| sp_set (X : SVar)
+| sp_const (sigma : Sigma)
+| sp_app (phi1 phi2 : Sigma_pattern)
+| sp_bottom
+| sp_impl (phi1 phi2 : Sigma_pattern)
+| sp_exists (x : EVar) (phi : Sigma_pattern)
+| sp_mu (X : SVar) (phi : Sigma_pattern)
 .
 
 (* Definition is_svar_box (s : SVar) : bool :=
-  match s with
-  | svar_c id => eqb id "box"
-  end
+match s with
+| svar_c id => eqb id "box"
+end
 .
 
 Inductive sp_context_e : Sigma_pattern -> Prop :=
-  | c_box (x : SVar) (p : (is_svar_box x) = true ) : sp_context_e (sp_set x)
-  | c_cons_l (spl spr : Sigma_pattern) (p : sp_context_e spl) : sp_context_e (sp_app spl spr)
-  | s_cons_r (spl spr : Sigma_pattern) (p : sp_context_e spr) : sp_context_e (sp_app spl spr)
+| c_box (x : SVar) (p : (is_svar_box x) = true ) :
+  sp_context_e (sp_set x)
+| c_cons_l (spl spr : Sigma_pattern) (p : sp_context_e spl) :
+  sp_context_e (sp_app spl spr)
+| s_cons_r (spl spr : Sigma_pattern) (p : sp_context_e spr) :
+  sp_context_e (sp_app spl spr)
 . *)
 
 Definition evar_eq_dec : forall (x y : EVar), { x = y } + { x <> y }.
@@ -44,132 +49,127 @@ Definition svar_eqb (x y : SVar) : bool := eqb (id_sv x) (id_sv y).
 Definition sigma_eqb (x y : Sigma) : bool := eqb (id_si x) (id_si y).
 
 Fixpoint spos_accumulated (phi : Sigma_pattern) (X : SVar) (nc : nat) : bool :=
-  match phi with
-  | sp_var x => true
-  | sp_set Y => if (svar_eq_dec Y X)
-                then (Nat.even nc)
-                else true
-  | sp_const sigma => true
-  | sp_app phi1 phi2 => andb (spos_accumulated phi1 X nc) (spos_accumulated phi2 X nc)
-  | sp_bottom => true
-  | sp_impl phi1 phi2 => andb (spos_accumulated phi1 X (S nc)) (spos_accumulated phi2 X nc)
-  | sp_exists x phi => spos_accumulated phi X nc
-  | sp_mu Y phi => if (svar_eq_dec Y X)
-                      then true
-                      else (spos_accumulated phi X nc)
+match phi with
+| sp_var x => true
+| sp_set Y => if (svar_eq_dec Y X)
+              then (Nat.even nc)
+              else true
+| sp_const sigma => true
+| sp_app phi1 phi2 => andb (spos_accumulated phi1 X nc)
+                           (spos_accumulated phi2 X nc)
+| sp_bottom => true
+| sp_impl phi1 phi2 => andb (spos_accumulated phi1 X (S nc))
+                            (spos_accumulated phi2 X nc)
+| sp_exists x phi => spos_accumulated phi X nc
+| sp_mu Y phi => if (svar_eq_dec Y X)
+                 then true
+                 else (spos_accumulated phi X nc)
 end.
 
-Fixpoint strictly_positive (phi : Sigma_pattern) (X : SVar) : bool :=  spos_accumulated phi X 0.
+Fixpoint strictly_positive (phi : Sigma_pattern) (X : SVar) : bool :=
+spos_accumulated phi X 0.
 
 Definition sp_eq_dec : forall (x y : Sigma_pattern), { x = y } + { x <> y }.
 Proof.
-  decide equality.
-  - exact (evar_eq_dec x0 x1).
-  - exact (svar_eq_dec X X0).
-  - exact (sigma_eq_dec sigma sigma0).
-  - exact (evar_eq_dec x0 x1).
-  - exact (svar_eq_dec X X0).
+decide equality.
+- exact (evar_eq_dec x0 x1).
+- exact (svar_eq_dec X X0).
+- exact (sigma_eq_dec sigma sigma0).
+- exact (evar_eq_dec x0 x1).
+- exact (svar_eq_dec X X0).
 Defined.
 
 Fixpoint e_subst_var (phi : Sigma_pattern) (psi : Sigma_pattern) (x : EVar) :=
-  match phi with
-  | sp_var x' =>
-      if evar_eq_dec x x'
-      then psi
-      else sp_var x'
-  | sp_set X => sp_set X
-  | sp_const sigma => sp_const sigma
-  | sp_app phi1 phi2 => sp_app (e_subst_var phi1 psi x)
-                                (e_subst_var phi2 psi x)
-  | sp_bottom => sp_bottom
-  | sp_impl phi1 phi2 => sp_impl (e_subst_var phi1 psi x)
-                                  (e_subst_var phi2 psi x)
-  | sp_exists x' phi' =>
-      if (evar_eq_dec x' x)
-      then sp_exists x' phi'
-      else sp_exists x' (e_subst_var phi' psi x)
-  | sp_mu X phi' => sp_mu X (e_subst_var phi' psi x)
+match phi with
+| sp_var x' => if evar_eq_dec x x'
+               then psi
+               else sp_var x'
+| sp_set X => sp_set X
+| sp_const sigma => sp_const sigma
+| sp_app phi1 phi2 => sp_app (e_subst_var phi1 psi x)
+                             (e_subst_var phi2 psi x)
+| sp_bottom => sp_bottom
+| sp_impl phi1 phi2 => sp_impl (e_subst_var phi1 psi x)
+                               (e_subst_var phi2 psi x)
+| sp_exists x' phi' => if (evar_eq_dec x' x)
+                       then sp_exists x' phi'
+                       else sp_exists x' (e_subst_var phi' psi x)
+| sp_mu X phi' => sp_mu X (e_subst_var phi' psi x)
 end.
 
 Fixpoint e_subst_set (phi : Sigma_pattern) (psi : Sigma_pattern) (X : SVar) :=
-  match phi with
-  | sp_var x => sp_var x
-  | sp_set X' =>
-      if svar_eq_dec X X'
-      then psi
-      else sp_set X'
-  | sp_const sigma => sp_const sigma
-  | sp_app phi1 phi2 => sp_app (e_subst_set phi1 psi X)
-                                (e_subst_set phi2 psi X)
-  | sp_bottom => sp_bottom
-  | sp_impl phi1 phi2 => sp_impl (e_subst_set phi1 psi X)
-                                  (e_subst_set phi2 psi X)
-  | sp_exists x' phi' => sp_exists x' (e_subst_set phi' psi X)
-  | sp_mu X' phi' =>
-      if (svar_eq_dec X' X)
-      then sp_mu X' phi'
-      else sp_mu X' (e_subst_set phi' psi X)
+match phi with
+| sp_var x => sp_var x
+| sp_set X' => if svar_eq_dec X X'
+               then psi
+               else sp_set X'
+| sp_const sigma => sp_const sigma
+| sp_app phi1 phi2 => sp_app (e_subst_set phi1 psi X)
+                             (e_subst_set phi2 psi X)
+| sp_bottom => sp_bottom
+| sp_impl phi1 phi2 => sp_impl (e_subst_set phi1 psi X)
+                               (e_subst_set phi2 psi X)
+| sp_exists x' phi' => sp_exists x' (e_subst_set phi' psi X)
+| sp_mu X' phi' => if (svar_eq_dec X' X)
+                   then sp_mu X' phi'
+                   else sp_mu X' (e_subst_set phi' psi X)
 end.
 
+(* Derived operators *)
 Definition sp_not (phi : Sigma_pattern) := sp_impl phi sp_bottom.
-Definition sp_or  (phi1 phi2 : Sigma_pattern) := sp_impl (sp_not phi1) phi2.
-Definition sp_and (phi1 phi2 : Sigma_pattern) :=
-  sp_not (sp_or (sp_not phi1) (sp_not phi2)).
-Definition sp_top := sp_not sp_bottom.
-Definition sp_only_if (phi1 phi2 : Sigma_pattern) := sp_and (sp_impl phi1 phi2) (sp_impl phi2 phi1).
-Definition sp_forall (x : EVar) (phi : Sigma_pattern) :=
-  sp_not (sp_exists x (sp_not phi)).
-Definition sp_nu (X : SVar) (phi : Sigma_pattern) := sp_not (sp_mu X (sp_not (e_subst_set phi (sp_not (sp_set X)) X))).
 
-Definition evar_eq (x y : EVar) : bool :=
-  match x, y with
-  | evar_c id_x, evar_c id_y => eqb id_x id_y
-  end
-.
+Definition sp_or  (phi1 phi2 : Sigma_pattern) := sp_impl (sp_not phi1) phi2.
+
+Definition sp_and (phi1 phi2 : Sigma_pattern) :=
+sp_not (sp_or (sp_not phi1) (sp_not phi2)).
+
+Definition sp_top := sp_not sp_bottom.
+
+Definition sp_only_if (phi1 phi2 : Sigma_pattern) :=
+sp_and (sp_impl phi1 phi2) (sp_impl phi2 phi1).
+
+Definition sp_forall (x : EVar) (phi : Sigma_pattern) :=
+sp_not (sp_exists x (sp_not phi)).
+
+Definition sp_nu (X : SVar) (phi : Sigma_pattern) :=
+sp_not (sp_mu X (sp_not (e_subst_set phi (sp_not (sp_set X)) X))).
+(*End of derived operators *)
 
 Fixpoint free_vars (phi : Sigma_pattern) : (set EVar) :=
-  match phi with
- | sp_var x => set_add evar_eq_dec x nil
- | sp_set X => nil
- | sp_const sigma => nil
- | sp_app phi1 phi2 =>
-    set_union evar_eq_dec
-      (free_vars phi1)
-      (free_vars phi2)
- | sp_bottom => nil
- | sp_impl phi1 phi2 =>
-    set_union evar_eq_dec
-      (free_vars phi1)
-      (free_vars phi2)
- | sp_exists y phi =>
-    set_diff evar_eq_dec
-      (free_vars phi)
-      (set_add evar_eq_dec y nil)
- | sp_mu X phi => free_vars phi
+match phi with
+| sp_var x => set_add evar_eq_dec x nil
+| sp_set X => nil
+| sp_const sigma => nil
+| sp_app phi1 phi2 => set_union evar_eq_dec (free_vars phi1) (free_vars phi2)
+| sp_bottom => nil
+| sp_impl phi1 phi2 => set_union evar_eq_dec (free_vars phi1) (free_vars phi2)
+| sp_exists y phi => set_diff evar_eq_dec (free_vars phi)
+                                          (set_add evar_eq_dec y nil)
+| sp_mu X phi => free_vars phi
 end
 .
 
 (* Definition is_free (x : EVar) (phi : Sigma_pattern) : bool :=
-  set_mem evar_eq_dec x (free_vars phi). *)
+set_mem evar_eq_dec x (free_vars phi). *)
 
 (* Inductive application_context : Set :=
-  | pattern (p : Sigma_pattern)
-  | box
+| pattern (p : Sigma_pattern)
+| box
 .
  *)
 
 Inductive context : Set :=
-  | box
-  | ctx_app_l (cc : context) (sp : Sigma_pattern)
-  | ctx_app_r (sp : Sigma_pattern) (cc : context)
+| box
+| ctx_app_l (cc : context) (sp : Sigma_pattern)
+| ctx_app_r (sp : Sigma_pattern) (cc : context)
 .
 
 Fixpoint subst_ctx (cc : context) (sp : Sigma_pattern) : Sigma_pattern :=
-  match cc with
-  | box => sp
-  | ctx_app_l cc' sp' => sp_app (subst_ctx cc' sp) sp'
-  | ctx_app_r sp' cc' => sp_app sp' (subst_ctx cc' sp)
-  end
+match cc with
+| box => sp
+| ctx_app_l cc' sp' => sp_app (subst_ctx cc' sp) sp'
+| ctx_app_r sp' cc' => sp_app sp' (subst_ctx cc' sp)
+end
 .
 
 (* FIXME Create Test File *)
@@ -182,130 +182,93 @@ Definition tree_context := subst_ctx (
 Eval compute in tree_context.
 
 Definition free_vars_ctx (C : context) : (set EVar) :=
-  match C with
-  | box => nil
-  | ctx_app_l cc sp => free_vars sp
-  | ctx_app_r sp cc => free_vars sp
-  end
+match C with
+| box => nil
+| ctx_app_l cc sp => free_vars sp
+| ctx_app_r sp cc => free_vars sp
+end
 .
 (* Inductive got_tau : Sigma_pattern -> Prop :=
   | cons (phi : Sigma_pattern) : got_tau (sp_impl sp_bottom phi)
 . *)
 
 Inductive got : Sigma_pattern -> Prop :=
-  (* Propositional tautology *)
-  (* | E_prop_tau phi : phi is prop tau -> got phi *)
+(* Propositional tautology *)
+(* | E_prop_tau phi : phi is prop tau -> got phi *)
 
-  (* Modus ponens *)
-  | E_mod_pon (phi1 phi2 : Sigma_pattern) :
-    got phi1 ->
-    got (sp_impl phi1 phi2) ->
-    got phi2
+(* Modus ponens *)
+| E_mod_pon (phi1 phi2 : Sigma_pattern) :
+  got phi1 ->
+  got (sp_impl phi1 phi2) ->
+  got phi2
 
-  (* Existential quantifier *)
-  | E_ex_quan {phi : Sigma_pattern} (x y : EVar) :
-    got (sp_impl (e_subst_var phi (sp_var y) x) (sp_exists x phi))
+(* Existential quantifier *)
+| E_ex_quan {phi : Sigma_pattern} (x y : EVar) :
+  got (sp_impl (e_subst_var phi (sp_var y) x) (sp_exists x phi))
 
-  (* Existential generalization *)
-  | E_ex_gen (phi1 phi2 : Sigma_pattern) (x : EVar) :
-    got (sp_impl phi1 phi2) ->
-    negb (set_mem evar_eq_dec x (free_vars phi2)) = true ->
-    got (sp_impl (sp_exists x phi1) phi2)
+(* Existential generalization *)
+| E_ex_gen (phi1 phi2 : Sigma_pattern) (x : EVar) :
+  got (sp_impl phi1 phi2) ->
+  negb (set_mem evar_eq_dec x (free_vars phi2)) = true ->
+  got (sp_impl (sp_exists x phi1) phi2)
 
-  (* Propagation bottom *)
-  | E_prop_bot (C : context) :
-    got (sp_impl (subst_ctx C sp_bottom) sp_bottom)
+(* Propagation bottom *)
+| E_prop_bot (C : context) :
+  got (sp_impl (subst_ctx C sp_bottom) sp_bottom)
 
-  (* Propagation disjunction *)
-  | E_prop_dis (C : context) (phi1 phi2 : Sigma_pattern) :
-      (* phi3 = context cs (sp_or phi1 phi2) ->
-      phi4 = context cs phi1 ->
-      phi5 = context cs phi2 ->
-      got_c (sp_impl phi3 (sp_or phi4 phi5)) *)
-      got (sp_impl
-            (subst_ctx C (sp_or phi1 phi2))
-            (sp_or
-              (subst_ctx C phi1)
-              (subst_ctx C phi2)))
-
-  (* Propagation exist *)
-  | E_prop_ex (C : context) (phi : Sigma_pattern) (x : EVar) :
-    negb (set_mem evar_eq_dec x (free_vars_ctx C)) = true ->
+(* Propagation disjunction *)
+| E_prop_dis (C : context) (phi1 phi2 : Sigma_pattern) :
+    (* phi3 = context cs (sp_or phi1 phi2) ->
+    phi4 = context cs phi1 ->
+    phi5 = context cs phi2 ->
+    got_c (sp_impl phi3 (sp_or phi4 phi5)) *)
     got (sp_impl
-      (subst_ctx C (sp_exists x phi))
-      (sp_exists x (subst_ctx C phi)))
+          (subst_ctx C (sp_or phi1 phi2))
+          (sp_or
+            (subst_ctx C phi1)
+            (subst_ctx C phi2)))
 
-  (* Framing *)
-  | E_framing (C : context) (phi1 phi2 : Sigma_pattern) :
-    got (sp_impl phi1 phi2) ->
-    got (sp_impl (subst_ctx C phi1) (subst_ctx C phi2))
+(* Propagation exist *)
+| E_prop_ex (C : context) (phi : Sigma_pattern) (x : EVar) :
+  negb (set_mem evar_eq_dec x (free_vars_ctx C)) = true ->
+  got (sp_impl
+    (subst_ctx C (sp_exists x phi))
+    (sp_exists x (subst_ctx C phi)))
 
-  (* Set Variable Substitution *)
-  | E_svar_subst (phi : Sigma_pattern) (psi X : SVar) :
-    got phi ->
-    got (e_subst_set phi (sp_set psi) X)
+(* Framing *)
+| E_framing (C : context) (phi1 phi2 : Sigma_pattern) :
+  got (sp_impl phi1 phi2) ->
+  got (sp_impl (subst_ctx C phi1) (subst_ctx C phi2))
 
-  (* Pre-Fixpoint *)
-  | E_pre_fixp (phi : Sigma_pattern) (X : SVar) :
-    got (sp_impl
-          (e_subst_set phi (sp_mu X phi) X)
-          (sp_mu X phi))
+(* Set Variable Substitution *)
+| E_svar_subst (phi : Sigma_pattern) (psi X : SVar) :
+  got phi ->
+  got (e_subst_set phi (sp_set psi) X)
 
-  (* Knaster-Tarski *)
-  | E_knaster_tarski (phi psi : Sigma_pattern) (X : SVar) :
-    got (sp_impl (e_subst_set phi psi X) psi) ->
-    got (sp_impl (sp_mu X phi) psi)
+(* Pre-Fixpoint *)
+| E_pre_fixp (phi : Sigma_pattern) (X : SVar) :
+  got (sp_impl
+        (e_subst_set phi (sp_mu X phi) X)
+        (sp_mu X phi))
 
-  (* Existence *)
-  | E_existence (x : EVar) : got (sp_exists x (sp_var x))
+(* Knaster-Tarski *)
+| E_knaster_tarski (phi psi : Sigma_pattern) (X : SVar) :
+  got (sp_impl (e_subst_set phi psi X) psi) ->
+  got (sp_impl (sp_mu X phi) psi)
 
-  (* Singleton *)
-  | E_singleton (C1 C2 : context) (x : EVar) (phi : Sigma_pattern) :
-    got (sp_not (sp_and
-            (subst_ctx C1 (sp_and (sp_var x) phi))
-            (subst_ctx C2 (sp_and (sp_var x) (sp_not phi)))))
+(* Existence *)
+| E_existence (x : EVar) : got (sp_exists x (sp_var x))
+
+(* Singleton *)
+| E_singleton (C1 C2 : context) (x : EVar) (phi : Sigma_pattern) :
+  got (sp_not (sp_and
+          (subst_ctx C1 (sp_and (sp_var x) phi))
+          (subst_ctx C2 (sp_and (sp_var x) (sp_not phi)))))
 .
 
-(* Inductive proof_result : ? :=
-  | success (?)
-  | fail
-. *)
-
-(* TO DO:
-    - free variables: Context -> Set OK
-    - eSubstitution for sets OK
-x occurs free
-x occurs bound
-instance of x is bound or not -> identify the location in the tree
-
-box, context : define inductively
- *)
-
-(*
-  2019.11.06.:
-  Context 3 fajtaja:
-    - inductive tipuskent OK
-    - az amit Daviddal most elkezdtunk () -
-    - a context egy fuggveny -
-  Folyamatosan jegyzeteljunk!
-*)
-(*
-  2019.11.13.:
-  - the best choice: context as a separate inductive type
-        reason: it is much simple to reason about an inductively defined structure, than to reason about a function of which we know nothing
-  - discuss about Gamma |- Phi  (soundness theorem)
-    - include it between proof rules
-*)
-
-End AML.
-
-Require Import Coq.Sets.Ensembles.
-Require Import Ensembles_Ext.
-
-Definition change_val {T1 T2 : Type} (eqb : T1 -> T1 -> bool) (t1 : T1) (t2 : T2) (f : T1 -> T2) : T1 -> T2 :=
-  fun x : T1 => if eqb x t1 then t2 else f x.
-
-Section Model.
+Definition change_val {T1 T2 : Type} (eqb : T1 -> T1 -> bool)
+                      (t1 : T1) (t2 : T2) (f : T1 -> T2) : T1 -> T2 :=
+fun x : T1 => if eqb x t1 then t2 else f x.
 
 Record Sigma_model := {
   M : Type;
@@ -314,36 +277,27 @@ Record Sigma_model := {
   interpretation : Sigma -> Ensemble M;
 }.
 
-Definition pointwise_app {sm : Sigma_model} (l r : Ensemble (M sm)) : Ensemble (M sm) :=
-  fun e:M sm => exists le re:M sm, l le -> r re -> (app sm) le re e.
+Definition pointwise_app {sm : Sigma_model} (l r : Ensemble (M sm)) :
+                         Ensemble (M sm) :=
+fun e:M sm => exists le re:M sm, l le -> r re -> (app sm) le re e.
 
-Fixpoint ext_valuation {sm : Sigma_model} (evar_val : EVar -> M sm) (svar_val : SVar -> Ensemble (M sm)) (sp : Sigma_pattern) : Ensemble (M sm) :=
+Fixpoint ext_valuation {sm : Sigma_model} (evar_val : EVar -> M sm)
+(svar_val : SVar -> Ensemble (M sm)) (sp : Sigma_pattern) : Ensemble (M sm) :=
 match sp with
-  (* sp_var *)
-  | sp_var x => Singleton _ (evar_val x)
-  (* sp_set *)
-  | sp_set X => svar_val X
-  (* sp_const *)
-  | sp_const s => (interpretation sm) s
-  (* sp_app *)
-  | sp_app ls rs =>
-    pointwise_app (ext_valuation evar_val svar_val ls) (ext_valuation evar_val svar_val rs)
-  (* sp_bottom *)
-  | sp_bottom => Empty_set _
-  (* sp_impl *)
-  | sp_impl ls rs => Union _ (Complement _ (ext_valuation evar_val svar_val ls)) (ext_valuation evar_val svar_val rs)
-  (* sp_exists *)
-  | sp_exists x sp =>
-    FA_Union (fun e => ext_valuation (change_val evar_eqb x e evar_val) svar_val sp)
-  (* sp_mu *)
-  | sp_mu X sp =>
-    mu (fun S => ext_valuation evar_val (change_val svar_eqb X S svar_val) sp)
+| sp_var x => Singleton _ (evar_val x)
+| sp_set X => svar_val X
+| sp_const s => (interpretation sm) s
+| sp_app ls rs => pointwise_app (ext_valuation evar_val svar_val ls)
+                                (ext_valuation evar_val svar_val rs)
+| sp_bottom => Empty_set _
+| sp_impl ls rs => Union _ (Complement _ (ext_valuation evar_val svar_val ls))
+                           (ext_valuation evar_val svar_val rs)
+| sp_exists x sp => FA_Union
+  (fun e => ext_valuation (change_val evar_eqb x e evar_val) svar_val sp)
+| sp_mu X sp => mu
+  (fun S => ext_valuation evar_val (change_val svar_eqb X S svar_val) sp)
 end
 .
-
-End Model.
-
-Require Import Ensembles_Ext.
 
 Ltac proof_ext_val :=
 simpl;intros;
@@ -351,7 +305,8 @@ repeat
   (* Normalize *)
    rewrite (Extensionality_Ensembles _ _ _ (Union_Empty_l _))
 || rewrite (Extensionality_Ensembles _ _ _ (Compl_Compl_Ensembles _ _))
-|| rewrite (Extensionality_Ensembles _ _ _ (Compl_Union_Coml_Intes_Ensembles _ _ _))
+|| rewrite
+   (Extensionality_Ensembles _ _ _ (Compl_Union_Coml_Intes_Ensembles _ _ _))
 || rewrite (Extensionality_Ensembles _ _ _ (FA_rel _ _ _))
   (* Apply *)
 || (eapply Same_set_Compl ; intros)
@@ -360,29 +315,57 @@ repeat
 || exact (Symdiff_val _ _)
 || exact (Same_set_refl _).
 
-Lemma not_ext_val_correct {sm : Sigma_model} {evar_val : EVar -> M sm} {svar_val : SVar -> Ensemble _} : forall sp : Sigma_pattern, Same_set _ (ext_valuation evar_val svar_val (sp_not sp)) (Complement _ (ext_valuation evar_val svar_val sp)).
+Lemma not_ext_val_correct
+{sm : Sigma_model} {evar_val : EVar -> M sm} {svar_val : SVar -> Ensemble _} :
+forall sp : Sigma_pattern, Same_set _
+  (ext_valuation evar_val svar_val (sp_not sp))
+  (Complement _ (ext_valuation evar_val svar_val sp)).
 Proof. proof_ext_val. Qed.
 
-Lemma or_ext_val_correct {sm : Sigma_model} {evar_val : EVar -> M sm} {svar_val : SVar -> Ensemble _} : forall spl spr : Sigma_pattern, Same_set _ (ext_valuation evar_val svar_val (sp_or spl spr)) (Union _ (ext_valuation evar_val svar_val spl) (ext_valuation evar_val svar_val spr)).
+Lemma or_ext_val_correct
+{sm : Sigma_model} {evar_val : EVar -> M sm} {svar_val : SVar -> Ensemble _} :
+forall spl spr : Sigma_pattern, Same_set _
+  (ext_valuation evar_val svar_val (sp_or spl spr))
+  (Union _ (ext_valuation evar_val svar_val spl)
+           (ext_valuation evar_val svar_val spr)).
 Proof. proof_ext_val. Qed.
 
-Lemma and_ext_val_correct {sm : Sigma_model} {evar_val : EVar -> M sm} {svar_val : SVar -> Ensemble _} : forall spl spr : Sigma_pattern, Same_set _ (ext_valuation evar_val svar_val (sp_and spl spr)) (Intersection _ (ext_valuation evar_val svar_val spl) (ext_valuation evar_val svar_val spr)).
+Lemma and_ext_val_correct
+{sm : Sigma_model} {evar_val : EVar -> M sm} {svar_val : SVar -> Ensemble _} :
+forall spl spr : Sigma_pattern, Same_set _
+  (ext_valuation evar_val svar_val (sp_and spl spr))
+  (Intersection _ (ext_valuation evar_val svar_val spl)
+                  (ext_valuation evar_val svar_val spr)).
 Proof. proof_ext_val. Qed.
 
-Lemma top_ext_val_correct {sm : Sigma_model} {evar_val : EVar -> M sm} {svar_val : SVar -> Ensemble _} : Same_set _ (ext_valuation evar_val svar_val (sp_top)) (Full_set _).
+Lemma top_ext_val_correct
+{sm : Sigma_model} {evar_val : EVar -> M sm} {svar_val : SVar -> Ensemble _} :
+Same_set _ (ext_valuation evar_val svar_val (sp_top)) (Full_set _).
 Proof. proof_ext_val. Qed.
 
-Lemma only_if_ext_val_correct {sm : Sigma_model} {evar_val : EVar -> M sm} {svar_val : SVar -> Ensemble _} : forall spl spr : Sigma_pattern, Same_set _ (ext_valuation evar_val svar_val (sp_only_if spl spr)) (Complement _ (Symmetric_difference (ext_valuation evar_val svar_val spl) (ext_valuation evar_val svar_val spr))).
+Lemma only_if_ext_val_correct
+{sm : Sigma_model} {evar_val : EVar -> M sm} {svar_val : SVar -> Ensemble _} :
+forall spl spr : Sigma_pattern, Same_set _
+  (ext_valuation evar_val svar_val (sp_only_if spl spr))
+  (Complement _ (Symmetric_difference (ext_valuation evar_val svar_val spl)
+                                      (ext_valuation evar_val svar_val spr))).
 Proof. proof_ext_val. Qed.
 
-Lemma forall_ext_val_correct {sm : Sigma_model} {evar_val : EVar -> M sm} {svar_val : SVar -> Ensemble _} : forall sp : Sigma_pattern, forall x : EVar, Same_set _ (ext_valuation evar_val svar_val (sp_forall x sp))
-(FA_Intersection (fun a:M sm => ext_valuation (change_val evar_eqb x a evar_val) svar_val sp)).
+Lemma forall_ext_val_correct
+{sm : Sigma_model} {evar_val : EVar -> M sm} {svar_val : SVar -> Ensemble _} :
+forall sp : Sigma_pattern, forall x : EVar, Same_set _
+  (ext_valuation evar_val svar_val (sp_forall x sp))
+  (FA_Intersection
+    (fun a => ext_valuation (change_val evar_eqb x a evar_val) svar_val sp)).
 Proof. proof_ext_val. eapply FA_Inters_same. intros. proof_ext_val. Qed.
 
-Lemma nu_ext_val_correct {sm : Sigma_model} {evar_val : EVar -> M sm} {svar_val : SVar -> Ensemble _} : forall sp : Sigma_pattern, forall X : SVar, Same_set _ (ext_valuation evar_val svar_val (sp_nu X sp))
-(nu (fun S => ext_valuation evar_val (change_val svar_eqb X S svar_val) sp)).
+Lemma nu_ext_val_correct
+{sm : Sigma_model} {evar_val : EVar -> M sm} {svar_val : SVar -> Ensemble _} :
+forall sp : Sigma_pattern, forall X : SVar, Same_set _
+  (ext_valuation evar_val svar_val (sp_nu X sp))
+  (nu (fun S => ext_valuation evar_val (change_val svar_eqb X S svar_val) sp)).
 Proof.
-proof_ext_val.
+(* proof_ext_val.
 unfold mu. unfold FA_Inters_cond.
 rewrite (Extensionality_Ensembles _ _ _ (FA_rel2 _ _ _)).
 unfold nu. unfold FA_Union_cond.
@@ -390,5 +373,7 @@ eapply FA_Union_same. intros.
 proof_ext_val.
 unfold Same_set. unfold Included. unfold Complement. unfold In. eapply conj.
 * intros. eapply conj.
-  - intros. unfold not in H.
+  - intros. unfold not in H. *)
 Admitted.
+
+End AML.
